src/program_proof/tulip/paxos/program/paxos_heartbeat_session.v
@@ -1,0 +1,35 @@
+From Perennial.program_proof.tulip.paxos Require Import prelude.
+From Perennial.program_proof.tulip.paxos.program Require Import repr.
+From Goose.github_com.mit_pdos.tulip Require Import paxos.
+
+Section program.
+  Context `{!heapGS Σ, !paxos_ghostG Σ}.
+
+  Theorem wp_Paxos__HeartbeatSession (px : loc) nidme γ :
+    is_paxos px nidme γ -∗
+    {{{ True }}}
+      Paxos__HeartbeatSession #px
+    {{{ RET #(); True }}}.
+  Proof.
+    iIntros "#Hpx" (Φ) "!> _ HΦ".
+    wp_rec.
+
+    (*@ func (px *Paxos) HeartbeatSession() {                                   @*)
+    (*@     for {                                                               @*)
+    (*@         primitive.Sleep(params.NS_HEARTBEAT_INTERVAL)                   @*)
+    (*@         px.cv.Broadcast()                                               @*)
+    (*@     }                                                                   @*)
+    (*@ }                                                                       @*)
+    wp_apply (wp_forBreak (λ _, True)%I); wp_pures; last by iApply "HΦ".
+    clear Φ.
+    iIntros (Φ) "!> _ HΦ".
+    wp_pures.
+    iNamed "Hpx".
+    wp_apply wp_Sleep.
+    wp_loadField.
+    wp_apply (wp_Cond__Broadcast with "Hcv").
+    wp_pures.
+    by iApply "HΦ".
+  Qed.
+
+End program.
