src/program_proof/tulip/program/gcoord/gcoord_attach.v
@@ -1,0 +1,29 @@
+From Perennial.program_proof.tulip.program Require Import prelude.
+From Perennial.program_proof.tulip.program.gcoord Require Import gcoord_repr.
+
+Section program.
+  Context `{!heapGS Σ, !tulip_ghostG Σ}.
+
+  Theorem wp_GroupCoordinator__Attach (gcoord : loc) (ts : u64) gid γ :
+    is_gcoord gcoord gid γ -∗
+    {{{ True }}}
+      GroupCoordinator__Attach #gcoord #ts
+    {{{ RET #(); True }}}.
+  Proof.
+    iIntros "#Hgcoord" (Φ) "!> _ HΦ".
+    wp_rec.
+
+    (*@ func (gcoord *GroupCoordinator) Attach(ts uint64) {                     @*)
+    (*@     gcoord.mu.Lock()                                                    @*)
+    (*@     gcoord.ts = ts                                                      @*)
+    (*@     gcoord.mu.Unlock()                                                  @*)
+    (*@ }                                                                       @*)
+    do 2 iNamed "Hgcoord".
+    wp_loadField.
+    wp_apply (wp_Mutex__Lock with "Hlock").
+    iIntros "[Hlocked Hgcoord]".
+    do 3 iNamed "Hgcoord". iNamed "Hts".
+    wp_storeField.
+  Admitted.
+
+End program.
