src/program_proof/tulip/program/gcoord/gpreparer_try_become_unpreparing.v
@@ -12,7 +12,7 @@ Section program.
     know_tulip_inv γ -∗
     {{{ own_gpreparer_with_phase gpp GPPValidating ts gid γ }}}
       GroupPreparer__tryBecomeUnpreparing #gpp
-    {{{ RET #(); own_gpreparer gpp ts gid γ }}}.
+    {{{ (resend : bool), RET #resend; own_gpreparer gpp ts gid γ }}}.
   Proof.
     iIntros (Hgid) "#Hinv".
     iIntros (Φ) "!> Hgpp HΦ".
