src/program_proof/tulip/program/replica/replica_request_session.v
@@ -693,43 +693,4 @@ Section program.
     }
   Qed.
 
-  Theorem wp_Replica__Serve (rp : loc) addr gid rid γ :
-    is_replica_plus_network rp addr gid rid γ -∗
-    {{{ True }}}
-      Replica__Serve #rp
-    {{{ RET #(); True }}}.
-  Proof.
-    iIntros "#Hrp" (Φ) "!> _ HΦ".
-    wp_rec.
-
-    (*@ func (rp *Replica) Serve() {                                            @*)
-    (*@     ls := grove_ffi.Listen(rp.addr)                                     @*)
-    (*@     for {                                                               @*)
-    (*@         conn := grove_ffi.Accept(ls)                                    @*)
-    (*@         go func() {                                                     @*)
-    (*@             rp.RequestSession(conn)                                     @*)
-    (*@         }()                                                             @*)
-    (*@     }                                                                   @*)
-    (*@ }                                                                       @*)
-    iNamed "Hrp".
-    wp_loadField.
-    wp_apply wp_Listen.
-    wp_pures.
-    wp_apply (wp_forBreak (λ _, True)%I); wp_pures; last by iApply "HΦ".
-    clear Φ.
-    iIntros (Φ) "!> _ HΦ".
-    wp_pures.
-    wp_apply wp_Accept.
-    iIntros (chanpeer) "_".
-    wp_pures.
-    wp_apply (wp_fork).
-    { (* Fork. *)
-      wp_apply wp_Replica__RequestSession.
-      { iFrame "# %". }
-      done.
-    }
-    wp_pures.
-    by iApply "HΦ".
-  Qed.
-
 End program.
