src/program_proof/tulip/program/replica/replica_serve.v
@@ -1,0 +1,48 @@
+From Perennial.program_proof.tulip.program Require Import prelude.
+From Perennial.program_proof.tulip.program.replica Require Import
+  replica_repr replica_request_session.
+From Perennial.program_proof.tulip.paxos Require Import base.
+
+Section program.
+  Context `{!heapGS Σ, !tulip_ghostG Σ, !paxos_ghostG Σ}.
+
+  Theorem wp_Replica__Serve (rp : loc) addr gid rid γ :
+    is_replica_plus_network rp addr gid rid γ -∗
+    {{{ True }}}
+      Replica__Serve #rp
+    {{{ RET #(); True }}}.
+  Proof.
+    iIntros "#Hrp" (Φ) "!> _ HΦ".
+    wp_rec.
+
+    (*@ func (rp *Replica) Serve() {                                            @*)
+    (*@     ls := grove_ffi.Listen(rp.addr)                                     @*)
+    (*@     for {                                                               @*)
+    (*@         conn := grove_ffi.Accept(ls)                                    @*)
+    (*@         go func() {                                                     @*)
+    (*@             rp.RequestSession(conn)                                     @*)
+    (*@         }()                                                             @*)
+    (*@     }                                                                   @*)
+    (*@ }                                                                       @*)
+    iNamed "Hrp".
+    wp_loadField.
+    wp_apply wp_Listen.
+    wp_pures.
+    wp_apply (wp_forBreak (λ _, True)%I); wp_pures; last by iApply "HΦ".
+    clear Φ.
+    iIntros (Φ) "!> _ HΦ".
+    wp_pures.
+    wp_apply wp_Accept.
+    iIntros (chanpeer) "_".
+    wp_pures.
+    wp_apply (wp_fork).
+    { (* Fork. *)
+      wp_apply wp_Replica__RequestSession.
+      { iFrame "# %". }
+      done.
+    }
+    wp_pures.
+    by iApply "HΦ".
+  Qed.
+
+End program.
